Revert "Partial work"
This reverts commit 218f853348eacaf6d56e0d1072afe28fdf48c922.

Source/DafnyStandardLibraries/src/Std/Actions/Producers.dfy
@@ -408,6 +408,8 @@ module Std.Producers {
     // there is no way to know if the consumer will accept a value ahead of time.
     // Therefore the producer may end up producing an extra value
     // that the consumer cannot accept, hence the extra leftover return value.
+    //
+    // TODO: Better name - Fill?
     method Fill(consumer: Consumer<T>, ghost totalActionProof: TotalActionProof<T, bool>)
       returns (leftover: Option<T>)
       requires Valid()
@@ -1719,7 +1721,7 @@ module Std.Producers {
     }
   }
 
-class MappedProducer<I, O> extends Producer<O> {
+  class MappedProducer<I, O> extends Producer<O> {
 
     const original: Producer<I>
     const mapping: Action<I, O>
@@ -1808,7 +1810,7 @@ class MappedProducer<I, O> extends Producer<O> {
     }
 
     @ResourceLimit("1e7")
-    method {:only} Invoke(t: ()) returns (result: Option<O>)
+    method Invoke(t: ()) returns (result: Option<O>)
       requires Requires(t)
       reads Reads(t)
       modifies Modifies(t)
@@ -1826,12 +1828,7 @@ class MappedProducer<I, O> extends Producer<O> {
         original.NewProducedAfterInvoke(next);
         assert original.NewProducedCount() == 1;
         mappingTotalProof.AnyInputIsValid(mapping.history, next.value);
-        label before:
-        assert {:only} unchanged(mapping.Repr);
         var nextValue := mapping.Invoke(next.value);
-        assert {:only} mapping.Ensures@before(next.value, nextValue);
-        assert {:only} mapping.ValidOutput@before(nextValue);
-        assert {:only} mapping.ValidOutput(nextValue);
         result := Some(nextValue);
 
         original.OutputtingSomeMeansAllSome(next.value);
@@ -1893,105 +1890,22 @@ class MappedProducer<I, O> extends Producer<O> {
     }
   }
 
-  trait OutputsNewProducersProof<I, O> {
-
-    ghost function Action(): Action<I, Producer<O>>
-
-    ghost function MaxProduced(): TerminationMetric
-
-    twostate lemma OutputFresh(new p: Producer<O>)
-      // requires Action().ValidChange()
-      requires Action().ValidOutput(p)
-      ensures 
-        && p.Valid()
-        && fresh(p.Repr)
-        && Action().Repr !! p.Repr
-        && p.history == []
-        && MaxProduced().DecreasesTo(p.DecreasesMetric())
-  }
-
-  @AssumeCrossModuleTermination
-  trait ProducerOfNewProducersProof<T> extends Validatable {
+  trait ProducerOfNewProducersProof<T> {
 
     ghost function Producer(): Producer<Producer<T>>
 
     ghost function MaxProduced(): TerminationMetric
 
-    twostate lemma ProducedFresh(new p: Producer<T>)
-      requires Valid()
+    twostate lemma JustProduced(new produced: Producer<T>)
       requires old(Producer().Requires(()))
       requires Producer().ValidChange()
-      requires Producer().Ensures((), Some(p))
+      requires Producer().Ensures((), Some(produced))
       ensures 
-        && p.Valid()
-        && fresh(p.Repr)
-        && Producer().Repr !! p.Repr
-        && p.history == []
-        && MaxProduced().DecreasesTo(p.DecreasesMetric())
-  }
-
-  class MappedProducerOfNewProducersProof<I, O> extends ProducerOfNewProducersProof<O> {
-
-    ghost const producer: MappedProducer<I, Producer<O>>
-    ghost const mappingProof: OutputsNewProducersProof<I, O>
-
-    constructor (ghost producer: MappedProducer<I, Producer<O>>,
-                  ghost mappingProof: OutputsNewProducersProof<I, O>)
-    {
-      this.producer := producer;
-      this.mappingProof := mappingProof;
-    }
-
-    ghost predicate Valid()
-      reads this, Repr
-      ensures Valid() ==> this in Repr
-      decreases Repr, 0
-    {
-      && this in Repr
-      && mappingProof.Action() == producer.mapping
-    }
-
-    twostate predicate ValidChange()
-      reads this, Repr
-      ensures ValidChange() ==>
-        old(Valid()) && Valid() && fresh(Repr - old(Repr))
-    {
-      old(Valid()) && Valid() && fresh(Repr - old(Repr))
-    }
-
-    twostate lemma ValidImpliesValidChange()
-      requires old(Valid())
-      requires unchanged(old(Repr))
-      ensures ValidChange()
-    {}
-
-    ghost function Producer(): Producer<Producer<O>>
-    {
-      producer
-    }
-
-    ghost function MaxProduced(): TerminationMetric {
-      mappingProof.MaxProduced()
-    }
-
-    twostate lemma {:only} ProducedFresh(new p: Producer<O>)
-      requires Valid()
-      requires old(Producer().Requires(()))
-      requires Producer().ValidChange()
-      requires Producer().Ensures((), Some(p))
-      ensures 
-        && p.Valid()
-        && fresh(p.Repr)
-        && Producer().Repr !! p.Repr
-        && p.history == []
-        && MaxProduced().DecreasesTo(p.DecreasesMetric())
-    {
-      assert producer.mapping.Valid();
-      assert producer.ValidOutput(Some(p));
-      assert producer.mapping.ValidOutput(p);
-      mappingProof.OutputFresh(p);
-    }
-
+        && produced.Valid()
+        && fresh(produced.Repr)
+        && Producer().Repr !! produced.Repr
+        && produced.history == []
+        && MaxProduced().DecreasesTo(produced.DecreasesMetric())
   }
 
   class FlattenedProducer<T> extends Producer<T> {
@@ -2014,7 +1928,7 @@ class MappedProducer<I, O> extends Producer<O> {
 
       this.originalProducesFreshProducers := originalProducesFreshProducers;
       this.history := [];
-      this.Repr := {this} + original.Repr + originalProducesFreshProducers.Repr;
+      this.Repr := {this} + original.Repr;
     }
 
     ghost function BaseMetric(): TerminationMetric
@@ -2102,8 +2016,7 @@ class MappedProducer<I, O> extends Producer<O> {
       && this in Repr
       && ValidComponent(original)
       && (currentInner.Some? ==> ValidComponent(currentInner.value))
-      && original.Repr !! (if currentInner.Some? then currentInner.value.Repr else {}) !! originalProducesFreshProducers.Repr
-      && ValidComponent(originalProducesFreshProducers)
+      && original.Repr !! (if currentInner.Some? then currentInner.value.Repr else {})
       && originalProducesFreshProducers.Producer() == original
       && ValidHistory(history)
       && (currentInner.Some? ==>
@@ -2164,9 +2077,6 @@ class MappedProducer<I, O> extends Producer<O> {
         invariant fresh(original.Repr - old(original.Repr))
         invariant currentInner.Some? ==> fresh(currentInner.value.Repr - old(Repr))
         invariant result.Some? ==> !original.Done() && currentInner.Some? && !currentInner.value.Done()
-        invariant originalProducesFreshProducers.Valid()
-        invariant originalProducesFreshProducers.Producer() == original
-        invariant original.Repr !!  (if currentInner.Some? then currentInner.value.Repr else {}) !! originalProducesFreshProducers.Repr
         invariant old(original.history) <= original.history
         invariant old(Done()) == Done()
         invariant DecreasedBy(result)
@@ -2182,8 +2092,8 @@ class MappedProducer<I, O> extends Producer<O> {
           assert fresh(original.Repr - old@beforeOriginalNext(Repr));
           if currentInner.Some? {
             assert original.ValidChange@beforeOriginalNext();
-            originalProducesFreshProducers.ProducedFresh@beforeOriginalNext(currentInner.value);
-            Repr := {this} + original.Repr + currentInner.value.Repr + originalProducesFreshProducers.Repr;
+            originalProducesFreshProducers.JustProduced@beforeOriginalNext(currentInner.value);
+            Repr := {this} + original.Repr + currentInner.value.Repr;
 
             assert ValidComponent(currentInner.value);
 
@@ -2198,7 +2108,7 @@ class MappedProducer<I, O> extends Producer<O> {
             old(DecreasesMetric()).TupleDecreasesToTuple(DecreasesMetric());
             assert old(Decreasing()) >= Decreasing();
           } else {
-            Repr := {this} + original.Repr + originalProducesFreshProducers.Repr;
+            Repr := {this} + original.Repr;
 
             assert currentInner == Seq.Last(original.Outputs());
             assert original.Done() && currentInner.None?;
@@ -2216,7 +2126,7 @@ class MappedProducer<I, O> extends Producer<O> {
           assert DecreasesMetric().second == TMSucc(currentInner.value.DecreasesMetric());
           DecreasesMetric().second.SuccDecreasesToOriginal();
           result := currentInner.value.Next();
-          this.Repr := {this} + original.Repr + currentInner.value.Repr + originalProducesFreshProducers.Repr;
+          this.Repr := {this} + original.Repr + currentInner.value.Repr;
 
           assert old@beforeCurrentInnerNext(currentInner.value.DecreasesMetric()).NonIncreasesTo(currentInner.value.DecreasesMetric());
           InnerDecreasesMetricNonIncreases@beforeCurrentInnerNext();
