Source/DafnyStandardLibraries/src/Std/Actions/Actions.dfy
@@ -43,13 +43,6 @@ module Std.Actions {
       requires ValidHistory(history)
       decreases Repr
 
-    twostate predicate ValidOutput(new o: O)
-      requires Valid()
-      decreases Repr
-    {
-      true
-    }
-
     ghost predicate Requires(i: I)
       reads Reads(i)
     {
@@ -72,7 +65,6 @@ module Std.Actions {
       reads Reads(i)
     {
       && ValidChange()
-      && ValidOutput(o)
       && history == old(history) + [(i, o)]
     }
 
